

Consider an input space  $X = \mathbb{R}^n$ . Suppose you have two scalar-valued constraints,  $h_1$  and  $h_2$ , which are satisfied if  $h_i = 0$ .

$$h_1(\mathbf{x}) \quad J_{h_1}(\mathbf{x}) = \nabla_{h_1}^T(\mathbf{x}) = \left[ \frac{\partial h_1}{\partial x_1} \quad \frac{\partial h_1}{\partial x_2} \quad \cdots \quad \frac{\partial h_1}{\partial x_n} \right]$$

$$h_2(\mathbf{x}) \quad J_{h_2}(\mathbf{x}) = \nabla_{h_2}^T(\mathbf{x}) = \left[ \frac{\partial h_2}{\partial x_1} \quad \frac{\partial h_2}{\partial x_2} \quad \cdots \quad \frac{\partial h_2}{\partial x_n} \right]$$

We want to combine these into one constraint, and then use Newton's method to project an input point  $\mathbf{x}_{in}$  onto the combined constraint.

One option is to stack the constraints into a vector-valued constraint function:

$$\mathbf{h}(\mathbf{x}) = \begin{bmatrix} h_1(\mathbf{x}) \\ h_2(\mathbf{x}) \end{bmatrix}$$

Then, apply Newton's method directly on  $\mathbf{h}$ :

$$\mathbf{h}_{\mathbf{p}}(\mathbf{x}) = \mathbf{h}(\mathbf{p}) + J_{\mathbf{h}}(\mathbf{p})(\mathbf{x} - \mathbf{p}) = \mathbf{0}$$

$$\mathbf{x} = \mathbf{p} - J_{\mathbf{h}}^{\dagger}(\mathbf{p}) \mathbf{h}(\mathbf{p})$$

with  $J^{\dagger}$  a left-inverse of  $J$ .

Alternatively, we could consider various ways of representing our constraint as a scalar-valued function  $s(\mathbf{x})$ . One common way is to use the  $\ell^2$  norm:

$$s(\mathbf{x}) = \|\mathbf{h}(\mathbf{x})\|$$

$$J_s(\mathbf{x}) = \nabla_s^T(\mathbf{x}) = \frac{\mathbf{h}^T(\mathbf{x})}{\|\mathbf{h}(\mathbf{x})\|} J_{\mathbf{h}}(\mathbf{x})$$

Applying Newton's method to  $\mathbf{s}$  yields:

$$\mathbf{x} = \mathbf{p} - \frac{1}{\|\nabla_s(\mathbf{x})\|^2} J_{\mathbf{h}}^T(\mathbf{p}) \mathbf{h}(\mathbf{x})$$

In other words, scalarizing the constraint using the  $\ell^2$  norm is equivalent to a Jacobian-transpose approach to root-finding.